new/proof/github_com/goose_lang/goose/testdata/examples/channel_search_replace.v
@@ -37,7 +37,7 @@ Definition waitgroupN := nroot .@ "waitgroup".
 
 Lemma wp_worker (γs: simple_names) (ch: loc) (wg: loc) (x y: w64) :
   {{{ is_pkg_init chan_spec_raw_examples ∗
-      "#Hchan" ∷ is_simple γs ch 4 (chanP wg x y) }}}
+      "#Hchan" ∷ is_simple γs ch (chanP wg x y) }}}
     @! chan_spec_raw_examples.worker #ch #wg #x #y
   {{{ RET #(); True }}}.
 Proof.
@@ -136,10 +136,10 @@ Proof using chan_protocolG0 waitgroup_joinG0 syncG0.
   }
   wp_apply chan.wp_make.
   { done. }
-  iIntros (ch γch_names) "[#His_chan Hoc]". simpl. wp_auto.
+  iIntros (ch γch_names) "(#His_chan & Hcap & Hoc)". simpl. wp_auto.
   iMod (init_WaitGroup with "wg") as (?) "H".
   iMod (join.init with "H") as "Hwg".
-  iMod (start_simple_buffered _ _ _ (chanP wg_ptr x y) with "[$His_chan] [$Hoc]") as (γch) "#Hchan".
+  iMod (start_simple_buffered _ _ (chanP wg_ptr x y) with "[$His_chan] [$Hoc]") as (γch) "#Hchan".
   iAssert (∃ (i : w64), "i" ∷ i_ptr ↦ i)%I with "[$i]" as "HH".
   wp_for. iNamed "HH". wp_auto.
   wp_if_destruct.
